deps/poulet4/lib/P4automata/Syntax.v
@@ -2,16 +2,55 @@ Require Coq.Lists.List.
 Import List.ListNotations.
 Require Coq.Logic.Eqdep_dec.
 Require Import Coq.Classes.EquivDec.
+Require Import Equations.Prop.EqDecInstances.
 Require Import Coq.Program.Program.
 Require Import Poulet4.HAList.
 Require Import Poulet4.FinType.
-Require Poulet4.P4cub.Envn.
+Require Poulet4.P4automata.DepEnv.
 Require Poulet4.P4automata.P4automaton.
 Module P4A := P4automaton.
 
-Module Env := Poulet4.P4cub.Envn.Env.
+Module Env := Poulet4.P4automata.DepEnv.
 
 Open Scope list_scope.
+
+Fixpoint n_tuple A (n: nat): Type :=
+  match n with
+  | 0 => unit
+  | S n => n_tuple A n * A
+  end.
+
+Fixpoint t2l A (n: nat) (x: n_tuple A n) : list A :=
+  match n as n' return n_tuple A n' -> list A with
+  | 0 => fun _ => []
+  | S n => fun p => t2l A n (fst p) ++ [snd p]
+  end x.
+
+Fixpoint n_tuple_app' {A n m} (xs: n_tuple A n) (ys: n_tuple A m) : n_tuple A (m + n) :=
+  match m as m' return (n_tuple A m' -> n_tuple A (m' + n)) with
+  | 0 =>
+    fun _ => xs
+  | S m0 =>
+    fun '(ys, y) => (n_tuple_app' xs ys, y)
+  end ys.
+
+Fixpoint n_tuple_repeat {A: Type} (n: nat) (a: A) : n_tuple A n :=
+  match n with
+  | 0 => tt
+  | S n => ((n_tuple_repeat n a), a)
+  end.
+
+Definition n_tuple_app {A n m} (xs: n_tuple A n) (ys: n_tuple A m) : n_tuple A (n + m).
+  rewrite Plus.plus_comm.
+  exact (n_tuple_app' xs ys).
+Defined.
+
+Program Instance n_tuple_eq_dec
+         {A: Type}
+         `{A_eq_dec: EquivDec.EqDec A eq}
+         (n: nat) : EquivDec.EqDec (n_tuple A n) eq.
+Next Obligation.
+Admitted.
 
 Section Syntax.
   Set Implicit Arguments.
@@ -58,64 +97,57 @@ Section Syntax.
         end }.
   Solve Obligations with unfold equiv, complement in *;
     program_simpl; congruence.
-  
-  Inductive expr :=
-  | EHdr (h: hdr_ref)
-  | ELit (bs: list bool)
-  | ESlice (e: expr) (hi lo: nat).
+
+  Inductive expr : nat -> Type :=
+  | EHdr {n} (h: H n): expr n
+  | ELit {n} (bs: n_tuple bool n): expr n
+  | ESlice {n} (e: expr n) (hi lo: nat): expr (Nat.min (1 + hi) n - lo).
   (* todo: binops, ...? *)
   
   Definition state_ref: Type := S + bool.
   
-  Inductive v :=
-  | VBits : list bool -> v.
+  Inductive v n :=
+  | VBits: n_tuple bool n -> v n.
 
-  Global Program Instance v_eq_dec : EquivDec.EqDec v eq :=
+  Global Program Instance v_eq_dec (n: nat): EquivDec.EqDec (v n) eq :=
     { equiv_dec x y :=
         match x, y with
-        | VBits xs, VBits ys =>
+        | VBits _ xs, VBits _ ys =>
           if xs == ys
           then in_left
           else in_right
         end }.
-  Solve Obligations with unfold equiv, complement in *;
+  Solve All Obligations with unfold equiv, complement in *;
     program_simpl; congruence.
 
-  Inductive pat :=
-  | PExact (val: v)
-  | PAny
-  | PPair (p1: pat) (p2: pat).
+  Inductive typ :=
+  | TBits (n: nat)
+  | TPair (t1 t2: typ).
 
-  Inductive cond :=
-  | CExpr (e: expr)
-  | CPair (c1: cond) (c2: cond).
+  Inductive pat: typ -> Type :=
+  | PExact {n} (val: v n) : pat (TBits n)
+  | PAny: forall n, pat (TBits n)
+  | PPair {t1 t2} (p1: pat t1) (p2: pat t2) : pat (TPair t1 t2).
 
-  Record sel_case: Type :=
-    { sc_pat: pat;
+  Inductive cond: typ -> Type :=
+  | CExpr {n} (e: expr n) : cond (TBits n)
+  | CPair {t1 t2} (c1: cond t1) (c2: cond t2) : cond (TPair t1 t2).
+
+  Record sel_case t: Type :=
+    { sc_pat: pat t;
       sc_st: state_ref }.
 
   Inductive transition: Type :=
   | TGoto (state: state_ref)
-  | TSel (c: cond) (cases: list sel_case) (default: state_ref).
+  | TSel {t} (c: cond t) (cases: list (sel_case t)) (default: state_ref).
 
-  Inductive op :=
-  | OpNil
-  | OpSeq (o1 o2: op)
-  | OpExtract (hdr: H')
-  | OpAsgn (lhs: H') (rhs: expr).
-  Arguments OpExtract : clear implicits.
-  Arguments OpAsgn : clear implicits.
+  Inductive op: nat -> Type :=
+  | OpNil: op 0
+  | OpSeq {n1 n2} (o1: op n1) (o2: op n2): op (n1 + n2)
+  | OpExtract (hdr: H'): op (projT1 hdr)
+  | OpAsgn {n} (lhs: H n) (rhs: expr n): op 0.
   
-  Fixpoint op_size (o: op) : nat :=
-    match o with
-    | OpNil => 0
-    | OpSeq o1 o2 =>
-      op_size o1 + op_size o2
-    | OpExtract h => projT1 h
-    | OpAsgn _ _ => 0
-    end.
-
-  Fixpoint nonempty (o: op) : Prop :=
+  Fixpoint nonempty {n} (o: op n) : Prop :=
     match o with
     | OpAsgn _ _
     | OpNil => True
@@ -124,11 +156,12 @@ Section Syntax.
     end.
 
   Record state: Type :=
-    { st_op: op;
+    { st_size: nat;
+      st_op: op st_size;
       st_trans: transition }.
 
   Definition state_size (st: state) : nat :=
-    op_size st.(st_op).
+    st_size st.
 
   Record t: Type :=
     { t_states: S -> state;
@@ -180,9 +213,9 @@ Section Fmap.
     | HRVar h => HRVar (sigma_fmapH h)
     end.
     
-  Fixpoint expr_fmapH (e: expr H1) : expr H2 :=
+  Fixpoint expr_fmapH {n} (e: expr H1 n) : expr H2 n :=
     match e with
-    | EHdr h => EHdr (hdr_ref_fmapH h)
+    | EHdr _ h => EHdr _ (g h)
     | ELit _ bs => ELit _ bs
     | ESlice e hi lo => ESlice (expr_fmapH e) hi lo
     end.
@@ -193,14 +226,14 @@ Section Fmap.
     | inr r => inr r
     end.
 
-  Definition sel_case_fmapS (c: sel_case S1) : sel_case S2 :=
+  Definition sel_case_fmapS {t} (c: sel_case S1 t) : sel_case S2 t :=
     {| sc_pat := c.(sc_pat);
        sc_st := state_ref_fmapS c.(sc_st) |}.
 
-  Fixpoint cond_fmapH (c: cond H1) : cond H2 :=
+  Fixpoint cond_fmapH {t} (c: cond H1 t) : cond H2 t :=
     match c with
-    | CExpr e => CExpr (expr_fmapH e)
-    | CPair c1 c2 => CPair (cond_fmapH c1) (cond_fmapH c2)
+    | @CExpr _ n e => CExpr (expr_fmapH e)
+    | @CPair _ t1 t2 c1 c2 => CPair (cond_fmapH c1) (cond_fmapH c2)
     end.
 
   Definition transition_fmapSH (t: transition S1 H1) : transition S2 H2 :=
@@ -210,35 +243,28 @@ Section Fmap.
       TSel (cond_fmapH cond) (List.map sel_case_fmapS cases) (state_ref_fmapS default)
     end.
 
-  Fixpoint op_fmapH (o: op H1) : op H2 :=
+  Fixpoint op_fmapH {n} (o: op H1 n) : op H2 n :=
     match o with
     | OpNil _ => OpNil _
     | OpSeq o1 o2 => OpSeq (op_fmapH o1) (op_fmapH o2)
     | OpExtract hdr => OpExtract (sigma_fmapH hdr)
-    | OpAsgn lhs rhs => OpAsgn (sigma_fmapH lhs) (expr_fmapH rhs)
+    | OpAsgn lhs rhs => OpAsgn (g lhs) (expr_fmapH rhs)
     end.
 
   Definition state_fmapSH (s: state S1 H1) : state S2 H2 :=
-    {| st_op := op_fmapH s.(st_op);
+    {| st_size := s.(st_size);
+       st_op := op_fmapH s.(st_op);
        st_trans := transition_fmapSH s.(st_trans) |}.
-
-  Lemma op_fmapH_size :
-    forall o,
-      op_size (op_fmapH o) = op_size o.
-  Proof.
-    induction o; simpl; eauto.
-  Qed.
 
   Lemma state_fmapSH_size :
     forall s,
       state_size (state_fmapSH s) = state_size s.
   Proof.
-    unfold state_size.
-    simpl; eauto using op_fmapH_size.
+    tauto.
   Qed.
 
   Lemma op_fmapH_nonempty :
-    forall o,
+    forall n (o: op H1 n),
       nonempty (op_fmapH o) <-> nonempty o.
   Proof.
     induction o; simpl; intuition.
@@ -258,54 +284,55 @@ Section Interp.
 
   Variable (a: t S H).
 
-  Definition store := Env.t (H' H) v.
+  Definition store := Env.t nat H v.
 
   Definition clamp_list (n: nat) (l: list bool) :=
     List.firstn n (l ++ (List.repeat false (List.length l - n))).
 
-  Definition clamp_v (n: nat) (x: v): v :=
-    match x with
-    | VBits x => VBits (clamp_list n x)
-    end.
-  
-  Definition assign (h: H' H) (v: v) (st: store) : store :=
-    Env.bind h (clamp_v (projT1 h) v) st.
+  Definition assign {n} (h: H n) (v: v n) (st: store) : store :=
+    Env.bind _ _ _ h v st.
 
-  Definition find (h: hdr_ref H) (st: store) : v :=
-    match h with
-    | HRVar x =>
-      match Env.find x st with
-      | Some v => v
-      | None => VBits nil
-      end
-    end.
+  Definition find {n} (h: H n) (st: store) : option (v n) :=
+    Env.find _ _ _ h st.
 
   Definition slice {A} (l: list A) (hi lo: nat) :=
     List.skipn lo (List.firstn (1 + hi) l).
 
-  Fixpoint eval_expr (st: store) (e: expr H) : v :=
-   match e with
-   | EHdr (HRVar x) =>
-     match Env.find x st with
-     | Some v => v
-     | None => VBits nil
-     end
-   | ELit _ bs =>
-     VBits bs
-   | ESlice e hi lo =>
-     let '(VBits bs) := eval_expr st e in
-     VBits (slice bs hi lo)
-   end.
+  Lemma slice_len:
+    forall A hi lo (l: list A),
+      length (slice l hi lo) = Nat.min (1 + hi) (length l) - lo.
+  Proof.
+    unfold slice.
+    intros.
+    rewrite List.skipn_length.
+    rewrite List.firstn_length.
+    reflexivity.
+  Qed.
+  
+  Definition n_slice {A n} (l: n_tuple A n) (hi lo: nat) : n_tuple A (Nat.min (1 + hi) n - lo).
+  Admitted. 
 
-  Fixpoint eval_op (st: store) (idx: nat) (bits: list bool) (o: op H) : store * nat :=
+  Equations eval_expr (n: nat) (st: store) (e: expr H n) : v n :=
+    { eval_expr st (EHdr n h) :=
+        match find h st with
+        | Some v => v
+        | None => VBits _ (n_tuple_repeat _ false)
+        end;
+      eval_expr st (ELit _ bs) := VBits _ bs;
+      eval_expr st (ESlice e hi lo) :=
+        let '(VBits _ bs) := eval_expr st e in
+        VBits _ (n_slice bs hi lo)
+    }.
+
+  Fixpoint eval_op {n size: nat} (st: store) (idx: nat) (bits: n_tuple bool n) (o: op H size) : store * n_tuple bool (n - size) :=
     match o with
-    | OpNil _ => (st, idx)
+    | OpNil _ => st
     | OpSeq o1 o2 =>
       let '(st, idx) := eval_op st idx bits o1 in
       eval_op st idx bits o2
     | OpExtract hdr =>
       let width := projT1 hdr in
-      (assign hdr (VBits (List.firstn width (List.skipn idx bits))) st, idx + width)
+      (assign (projT2 hdr) (VBits _ (List.firstn width (List.skipn idx bits))) st, idx + width)
     | OpAsgn hdr expr =>
       (assign hdr (eval_expr st expr) st, idx)
     end.
